src/PermAsyncDisk.v
@@ -97,6 +97,13 @@ Definition valuset := (tagged_block * list tagged_block)%type.
 Definition tagged_block0 := (Public, natToWord valulen 0).
 Definition valuset0 := (tagged_block0, nil:list tagged_block). 
 
+Definition tagged_block_dec : forall (t t': tagged_block), {t = t'}+{t <> t'}.
+  intros; destruct t, t'; simpl.
+  destruct (tag_dec t t0); subst;
+  auto; try solve [right; congruence].
+  destruct (weq b b0); subst;
+  auto; try solve [right; congruence].
+Defined.
 
 (* Async-disk *)
 Definition rawdisk := @mem addr addr_eq_dec valuset.
