src/PermProg.v
@@ -39,8 +39,8 @@ Axiom can_access: perm -> tag -> Prop.
 Axiom can_access_public: forall pr, can_access pr Public.
 Hint Resolve can_access_public.
 
-Inductive result : Type :=
-| Finished : forall T, tagged_disk -> block_mem -> hashmap -> T -> result
+Inductive result {T: Type} : Type :=
+| Finished : tagged_disk -> block_mem -> hashmap -> T -> result
 | Crashed : tagged_disk -> block_mem -> hashmap -> result.
 
 Inductive prog : Type -> Type :=
@@ -60,7 +60,7 @@ Inductive prog : Type -> Type :=
 
 Inductive exec:
   forall T, perm -> trace -> tagged_disk ->
-       block_mem -> hashmap -> prog T ->  result -> trace -> Prop :=
+       block_mem -> hashmap -> prog T ->  @result T -> trace -> Prop :=
 | ExecRead    : forall pr d bm hm a i tb tbs tr,
                   bm i = None ->
                   d a = Some (tb, tbs) ->
@@ -132,10 +132,9 @@ Inductive exec:
 | CrashSync : forall pr d bm hm tr,
                 exec pr tr d bm hm (Sync) (Crashed d bm hm) tr
 
-| CrashBind : forall T T' pr (p1 : prog T) (p2: T -> prog T') d d' bm bm' hm hm' tr tr' r,
-                exec pr tr d bm hm p1 r tr' ->
-                r = (Crashed d' bm' hm') ->
-                exec pr tr d bm hm (Bind p1 p2) r tr'.
+| CrashBind : forall T T' pr (p1 : prog T) (p2: T -> prog T') d d' bm bm' hm hm' tr tr',
+                exec pr tr d bm hm p1 (@Crashed T d' bm' hm') tr' ->
+                exec pr tr d bm hm (Bind p1 p2) (@Crashed T' d' bm' hm') tr'.
 
 
 
